<?xml version="1.0"?>
<rdf:RDF xmlns="https://raw.githubusercontent.com/carrineblank/MicrO/master/MicrOandImportModules/PO_imports.owl#"
     xml:base="https://raw.githubusercontent.com/carrineblank/MicrO/master/MicrOandImportModules/PO_imports.owl"
     xmlns:po="http://purl.obolibrary.org/obo/po#"
     xmlns:obo="http://purl.obolibrary.org/obo/"
     xmlns:owl="http://www.w3.org/2002/07/owl#"
     xmlns:rdf="http://www.w3.org/1999/02/22-rdf-syntax-ns#"
     xmlns:xml="http://www.w3.org/XML/1998/namespace"
     xmlns:xsd="http://www.w3.org/2001/XMLSchema#"
     xmlns:rdfs="http://www.w3.org/2000/01/rdf-schema#"
     xmlns:oboInOwl="http://www.geneontology.org/formats/oboInOwl#">
    <owl:Ontology rdf:about="https://raw.githubusercontent.com/carrineblank/MicrO/master/MicrOandImportModules/PO_imports.owl"/>
    


    <!-- 
    ///////////////////////////////////////////////////////////////////////////////////////
    //
    // Annotation properties
    //
    ///////////////////////////////////////////////////////////////////////////////////////
     -->

    


    <!-- http://purl.obolibrary.org/obo/IAO_0000115 -->

    <owl:AnnotationProperty rdf:about="http://purl.obolibrary.org/obo/IAO_0000115">
        <rdfs:label>definition</rdfs:label>
    </owl:AnnotationProperty>
    


    <!-- http://purl.obolibrary.org/obo/IAO_0000412 -->

    <owl:AnnotationProperty rdf:about="http://purl.obolibrary.org/obo/IAO_0000412">
        <rdfs:label xml:lang="en">imported from</rdfs:label>
    </owl:AnnotationProperty>
    


    <!-- http://purl.obolibrary.org/obo/po#Gymnosperms -->

    <owl:AnnotationProperty rdf:about="http://purl.obolibrary.org/obo/po#Gymnosperms"/>
    


    <!-- http://purl.obolibrary.org/obo/po#Maize -->

    <owl:AnnotationProperty rdf:about="http://purl.obolibrary.org/obo/po#Maize"/>
    


    <!-- http://purl.obolibrary.org/obo/po#Poaceae -->

    <owl:AnnotationProperty rdf:about="http://purl.obolibrary.org/obo/po#Poaceae"/>
    


    <!-- http://purl.obolibrary.org/obo/po#Potato -->

    <owl:AnnotationProperty rdf:about="http://purl.obolibrary.org/obo/po#Potato"/>
    


    <!-- http://purl.obolibrary.org/obo/po#Rice -->

    <owl:AnnotationProperty rdf:about="http://purl.obolibrary.org/obo/po#Rice"/>
    


    <!-- http://purl.obolibrary.org/obo/po#Tomato -->

    <owl:AnnotationProperty rdf:about="http://purl.obolibrary.org/obo/po#Tomato"/>
    


    <!-- http://purl.obolibrary.org/obo/po#TraitNet -->

    <owl:AnnotationProperty rdf:about="http://purl.obolibrary.org/obo/po#TraitNet"/>
    


    <!-- http://purl.obolibrary.org/obo/po#reference -->

    <owl:AnnotationProperty rdf:about="http://purl.obolibrary.org/obo/po#reference"/>
    


    <!-- http://www.geneontology.org/formats/oboInOwl#created_by -->

    <owl:AnnotationProperty rdf:about="http://www.geneontology.org/formats/oboInOwl#created_by"/>
    


    <!-- http://www.geneontology.org/formats/oboInOwl#creation_date -->

    <owl:AnnotationProperty rdf:about="http://www.geneontology.org/formats/oboInOwl#creation_date"/>
    


    <!-- http://www.geneontology.org/formats/oboInOwl#hasAlternativeId -->

    <owl:AnnotationProperty rdf:about="http://www.geneontology.org/formats/oboInOwl#hasAlternativeId">
        <rdfs:label>has_alternative_id</rdfs:label>
    </owl:AnnotationProperty>
    


    <!-- http://www.geneontology.org/formats/oboInOwl#hasBroadSynonym -->

    <owl:AnnotationProperty rdf:about="http://www.geneontology.org/formats/oboInOwl#hasBroadSynonym">
        <rdfs:label>has_broad_synonym</rdfs:label>
    </owl:AnnotationProperty>
    


    <!-- http://www.geneontology.org/formats/oboInOwl#hasDbXref -->

    <owl:AnnotationProperty rdf:about="http://www.geneontology.org/formats/oboInOwl#hasDbXref">
        <rdfs:label>database_cross_reference</rdfs:label>
    </owl:AnnotationProperty>
    


    <!-- http://www.geneontology.org/formats/oboInOwl#hasExactSynonym -->

    <owl:AnnotationProperty rdf:about="http://www.geneontology.org/formats/oboInOwl#hasExactSynonym">
        <rdfs:label>has_exact_synonym</rdfs:label>
    </owl:AnnotationProperty>
    


    <!-- http://www.geneontology.org/formats/oboInOwl#hasNarrowSynonym -->

    <owl:AnnotationProperty rdf:about="http://www.geneontology.org/formats/oboInOwl#hasNarrowSynonym">
        <rdfs:label>has_narrow_synonym</rdfs:label>
    </owl:AnnotationProperty>
    


    <!-- http://www.geneontology.org/formats/oboInOwl#hasOBONamespace -->

    <owl:AnnotationProperty rdf:about="http://www.geneontology.org/formats/oboInOwl#hasOBONamespace">
        <rdfs:label>has_obo_namespace</rdfs:label>
    </owl:AnnotationProperty>
    


    <!-- http://www.geneontology.org/formats/oboInOwl#hasRelatedSynonym -->

    <owl:AnnotationProperty rdf:about="http://www.geneontology.org/formats/oboInOwl#hasRelatedSynonym">
        <rdfs:label>has_related_synonym</rdfs:label>
    </owl:AnnotationProperty>
    


    <!-- http://www.geneontology.org/formats/oboInOwl#id -->

    <owl:AnnotationProperty rdf:about="http://www.geneontology.org/formats/oboInOwl#id"/>
    


    <!-- http://www.geneontology.org/formats/oboInOwl#inSubset -->

    <owl:AnnotationProperty rdf:about="http://www.geneontology.org/formats/oboInOwl#inSubset">
        <rdfs:label>in_subset</rdfs:label>
    </owl:AnnotationProperty>
    


    <!-- 
    ///////////////////////////////////////////////////////////////////////////////////////
    //
    // Object Properties
    //
    ///////////////////////////////////////////////////////////////////////////////////////
     -->

    


    <!-- http://purl.obolibrary.org/obo/BFO_0000050 -->

    <owl:ObjectProperty rdf:about="http://purl.obolibrary.org/obo/BFO_0000050">
        <rdf:type rdf:resource="http://www.w3.org/2002/07/owl#TransitiveProperty"/>
        <rdfs:label>part_of</rdfs:label>
    </owl:ObjectProperty>
    


    <!-- http://purl.obolibrary.org/obo/BFO_0000051 -->

    <owl:ObjectProperty rdf:about="http://purl.obolibrary.org/obo/BFO_0000051">
        <rdf:type rdf:resource="http://www.w3.org/2002/07/owl#TransitiveProperty"/>
        <rdfs:label>has_part</rdfs:label>
    </owl:ObjectProperty>
    


    <!-- http://purl.obolibrary.org/obo/RO_0002202 -->

    <owl:ObjectProperty rdf:about="http://purl.obolibrary.org/obo/RO_0002202">
        <rdf:type rdf:resource="http://www.w3.org/2002/07/owl#TransitiveProperty"/>
        <rdfs:label>develops_from</rdfs:label>
    </owl:ObjectProperty>
    


    <!-- 
    ///////////////////////////////////////////////////////////////////////////////////////
    //
    // Classes
    //
    ///////////////////////////////////////////////////////////////////////////////////////
     -->

    


    <!-- http://purl.obolibrary.org/obo/PO_0000003 -->

    <owl:Class rdf:about="http://purl.obolibrary.org/obo/PO_0000003">
        <rdfs:subClassOf rdf:resource="http://purl.obolibrary.org/obo/PO_0009011"/>
        <obo:IAO_0000115>A plant structure (PO:0005679) which is a whole organism.</obo:IAO_0000115>
        <obo:IAO_0000412 rdf:resource="http://purl.obolibrary.org/obo/po.owl"/>
        <oboInOwl:hasBroadSynonym>genet</oboInOwl:hasBroadSynonym>
        <oboInOwl:hasBroadSynonym>ramet</oboInOwl:hasBroadSynonym>
        <oboInOwl:hasDbXref>OBO_SF_PO:2968335</oboInOwl:hasDbXref>
        <oboInOwl:hasDbXref>OBO_SF_PO:3612743</oboInOwl:hasDbXref>
        <oboInOwl:hasExactSynonym>planta entera (Spanish)</oboInOwl:hasExactSynonym>
        <oboInOwl:hasExactSynonym>植物体全体 (Japanese)</oboInOwl:hasExactSynonym>
        <oboInOwl:hasNarrowSynonym>bush</oboInOwl:hasNarrowSynonym>
        <oboInOwl:hasNarrowSynonym>frutex</oboInOwl:hasNarrowSynonym>
        <oboInOwl:hasNarrowSynonym>frutices</oboInOwl:hasNarrowSynonym>
        <oboInOwl:hasNarrowSynonym>gametophyte</oboInOwl:hasNarrowSynonym>
        <oboInOwl:hasNarrowSynonym>herb</oboInOwl:hasNarrowSynonym>
        <oboInOwl:hasNarrowSynonym>liana</oboInOwl:hasNarrowSynonym>
        <oboInOwl:hasNarrowSynonym>prothalli</oboInOwl:hasNarrowSynonym>
        <oboInOwl:hasNarrowSynonym>prothallium</oboInOwl:hasNarrowSynonym>
        <oboInOwl:hasNarrowSynonym>prothallus</oboInOwl:hasNarrowSynonym>
        <oboInOwl:hasNarrowSynonym>seedling</oboInOwl:hasNarrowSynonym>
        <oboInOwl:hasNarrowSynonym>shrub</oboInOwl:hasNarrowSynonym>
        <oboInOwl:hasNarrowSynonym>sporophyte</oboInOwl:hasNarrowSynonym>
        <oboInOwl:hasNarrowSynonym>suffrutex</oboInOwl:hasNarrowSynonym>
        <oboInOwl:hasNarrowSynonym>suffrutices</oboInOwl:hasNarrowSynonym>
        <oboInOwl:hasNarrowSynonym>tree</oboInOwl:hasNarrowSynonym>
        <oboInOwl:hasNarrowSynonym>vine</oboInOwl:hasNarrowSynonym>
        <oboInOwl:hasNarrowSynonym>woody clump</oboInOwl:hasNarrowSynonym>
        <oboInOwl:hasOBONamespace>plant_anatomy</oboInOwl:hasOBONamespace>
        <oboInOwl:hasRelatedSynonym>clonal colony</oboInOwl:hasRelatedSynonym>
        <oboInOwl:hasRelatedSynonym>colony</oboInOwl:hasRelatedSynonym>
        <oboInOwl:id>PO:0000003</oboInOwl:id>
        <oboInOwl:inSubset rdf:resource="http://purl.obolibrary.org/obo/po#TraitNet"/>
        <oboInOwl:inSubset rdf:resource="http://purl.obolibrary.org/obo/po#reference"/>
        <rdfs:comment>Examples include plant embryo (PO:0009009), megagametophyte (PO:0025279) and microgametophyte (PO:0025280).</rdfs:comment>
        <rdfs:label>whole plant</rdfs:label>
    </owl:Class>
    


    <!-- http://purl.obolibrary.org/obo/PO_0004543 -->

    <owl:Class rdf:about="http://purl.obolibrary.org/obo/PO_0004543">
        <rdfs:subClassOf rdf:resource="http://purl.obolibrary.org/obo/PO_0025522"/>
        <obo:IAO_0000115>A tuber (PO:0025522) that develops from a branch (PO:0025073).</obo:IAO_0000115>
        <obo:IAO_0000412 rdf:resource="http://purl.obolibrary.org/obo/po.owl"/>
        <oboInOwl:hasBroadSynonym>diaspore</oboInOwl:hasBroadSynonym>
        <oboInOwl:hasDbXref>OBO_SF_PO:3017726</oboInOwl:hasDbXref>
        <oboInOwl:hasExactSynonym>shoot axis branch tuber</oboInOwl:hasExactSynonym>
        <oboInOwl:hasExactSynonym>tub&amp;#233rculo (Spanish)</oboInOwl:hasExactSynonym>
        <oboInOwl:hasExactSynonym>tuber branch</oboInOwl:hasExactSynonym>
        <oboInOwl:hasExactSynonym>シュート軸塊茎 (Japanese)</oboInOwl:hasExactSynonym>
        <oboInOwl:hasOBONamespace>plant_anatomy</oboInOwl:hasOBONamespace>
        <oboInOwl:id>PO:0004543</oboInOwl:id>
        <oboInOwl:inSubset rdf:resource="http://purl.obolibrary.org/obo/po#Potato"/>
        <oboInOwl:inSubset rdf:resource="http://purl.obolibrary.org/obo/po#TraitNet"/>
        <oboInOwl:inSubset rdf:resource="http://purl.obolibrary.org/obo/po#reference"/>
        <rdfs:comment>Functions in storage of photosynthate metabolites. This term should be used for tubers derived from branches, as found in Solanum spp. (e.g. potato) or Dioscorea spp. (e.g. yam) and other species. Use the term tuberous root tuber (PO:0025476) for tubers derived from roots, such as those found in Cassava, Ipomoea, or Hemerocallis.</rdfs:comment>
        <rdfs:label>shoot axis tuber</rdfs:label>
    </owl:Class>
    


    <!-- http://purl.obolibrary.org/obo/PO_0004547 -->

    <owl:Class rdf:about="http://purl.obolibrary.org/obo/PO_0004547">
        <rdfs:subClassOf rdf:resource="http://purl.obolibrary.org/obo/PO_0004543"/>
        <obo:IAO_0000115>A shoot axis tuber (PO:0004543) that develops below ground.</obo:IAO_0000115>
        <obo:IAO_0000412 rdf:resource="http://purl.obolibrary.org/obo/po.owl"/>
        <oboInOwl:hasExactSynonym>tub&amp;#233rculo subterr&amp;#225neo (Spanish)</oboInOwl:hasExactSynonym>
        <oboInOwl:hasExactSynonym>地下塊茎 (Japanese)</oboInOwl:hasExactSynonym>
        <oboInOwl:hasOBONamespace>plant_anatomy</oboInOwl:hasOBONamespace>
        <oboInOwl:id>PO:0004547</oboInOwl:id>
        <oboInOwl:inSubset rdf:resource="http://purl.obolibrary.org/obo/po#Potato"/>
        <rdfs:comment>Functions in storage of photosynthate metabolites. This term should be used for tubers derived from branches, as found in Solanum spp. (e.g. potato) or Dioscorea spp. (e.g. yam) and other species. Use the term tuberous root tuber (PO:0025476) for tubers derived from roots, such as those found in Cassava, Ipomoea, or Hemerocallis.</rdfs:comment>
        <rdfs:label>subterranean tuber</rdfs:label>
    </owl:Class>
    


    <!-- http://purl.obolibrary.org/obo/PO_0006001 -->

    <owl:Class rdf:about="http://purl.obolibrary.org/obo/PO_0006001">
        <rdfs:subClassOf rdf:resource="http://purl.obolibrary.org/obo/PO_0009008"/>
        <obo:IAO_0000115>A lateral plant organ (PO:0009008) produced by a shoot apical meristem (PO:0020148).</obo:IAO_0000115>
        <obo:IAO_0000412 rdf:resource="http://purl.obolibrary.org/obo/po.owl"/>
        <oboInOwl:hasExactSynonym>filoma (Spanish)</oboInOwl:hasExactSynonym>
        <oboInOwl:hasExactSynonym>フィロム、葉(的）器官 (Japanese)</oboInOwl:hasExactSynonym>
        <oboInOwl:hasOBONamespace>plant_anatomy</oboInOwl:hasOBONamespace>
        <oboInOwl:id>PO:0006001</oboInOwl:id>
        <oboInOwl:inSubset rdf:resource="http://purl.obolibrary.org/obo/po#TraitNet"/>
        <oboInOwl:inSubset rdf:resource="http://purl.obolibrary.org/obo/po#reference"/>
        <rdfs:label>phyllome</rdfs:label>
    </owl:Class>
    


    <!-- http://purl.obolibrary.org/obo/PO_0009001 -->

    <owl:Class rdf:about="http://purl.obolibrary.org/obo/PO_0009001">
        <rdfs:subClassOf rdf:resource="http://purl.obolibrary.org/obo/PO_0025496"/>
        <obo:IAO_0000115>A multi-tissue plant structure (PO:0025496) that develops from a gynoecium (PO:0009062) and may have as parts one or more seeds (PO:0009010).</obo:IAO_0000115>
        <obo:IAO_0000412 rdf:resource="http://purl.obolibrary.org/obo/po.owl"/>
        <oboInOwl:hasAlternativeId>PO:0020067</oboInOwl:hasAlternativeId>
        <oboInOwl:hasAlternativeId>PO:0020068</oboInOwl:hasAlternativeId>
        <oboInOwl:hasAlternativeId>PO:0020069</oboInOwl:hasAlternativeId>
        <oboInOwl:hasAlternativeId>PO:0020070</oboInOwl:hasAlternativeId>
        <oboInOwl:hasAlternativeId>PO:0020071</oboInOwl:hasAlternativeId>
        <oboInOwl:hasAlternativeId>PO:0020072</oboInOwl:hasAlternativeId>
        <oboInOwl:hasAlternativeId>PO:0020073</oboInOwl:hasAlternativeId>
        <oboInOwl:hasAlternativeId>PO:0020074</oboInOwl:hasAlternativeId>
        <oboInOwl:hasAlternativeId>PO:0020076</oboInOwl:hasAlternativeId>
        <oboInOwl:hasAlternativeId>PO:0020077</oboInOwl:hasAlternativeId>
        <oboInOwl:hasAlternativeId>PO:0020078</oboInOwl:hasAlternativeId>
        <oboInOwl:hasAlternativeId>PO:0020079</oboInOwl:hasAlternativeId>
        <oboInOwl:hasAlternativeId>PO:0020080</oboInOwl:hasAlternativeId>
        <oboInOwl:hasAlternativeId>PO:0020082</oboInOwl:hasAlternativeId>
        <oboInOwl:hasAlternativeId>PO:0020083</oboInOwl:hasAlternativeId>
        <oboInOwl:hasAlternativeId>PO:0020087</oboInOwl:hasAlternativeId>
        <oboInOwl:hasAlternativeId>PO:0020107</oboInOwl:hasAlternativeId>
        <oboInOwl:hasBroadSynonym>diaspore</oboInOwl:hasBroadSynonym>
        <oboInOwl:hasDbXref>OBO_SF_PO:2972169</oboInOwl:hasDbXref>
        <oboInOwl:hasExactSynonym>fruto (Spanish)</oboInOwl:hasExactSynonym>
        <oboInOwl:hasExactSynonym>果実 (Japanese)</oboInOwl:hasExactSynonym>
        <oboInOwl:hasNarrowSynonym>accessory fruit</oboInOwl:hasNarrowSynonym>
        <oboInOwl:hasNarrowSynonym>achene</oboInOwl:hasNarrowSynonym>
        <oboInOwl:hasNarrowSynonym>acorn</oboInOwl:hasNarrowSynonym>
        <oboInOwl:hasNarrowSynonym>aggregate fruit</oboInOwl:hasNarrowSynonym>
        <oboInOwl:hasNarrowSynonym>akene</oboInOwl:hasNarrowSynonym>
        <oboInOwl:hasNarrowSynonym>anthocarp</oboInOwl:hasNarrowSynonym>
        <oboInOwl:hasNarrowSynonym>berry</oboInOwl:hasNarrowSynonym>
        <oboInOwl:hasNarrowSynonym>capsule</oboInOwl:hasNarrowSynonym>
        <oboInOwl:hasNarrowSynonym>caryopsides</oboInOwl:hasNarrowSynonym>
        <oboInOwl:hasNarrowSynonym>caryopsis</oboInOwl:hasNarrowSynonym>
        <oboInOwl:hasNarrowSynonym>circumcissile capsule</oboInOwl:hasNarrowSynonym>
        <oboInOwl:hasNarrowSynonym>citrus fruit</oboInOwl:hasNarrowSynonym>
        <oboInOwl:hasNarrowSynonym>coenocarp</oboInOwl:hasNarrowSynonym>
        <oboInOwl:hasNarrowSynonym>cypsela</oboInOwl:hasNarrowSynonym>
        <oboInOwl:hasNarrowSynonym>diclesia</oboInOwl:hasNarrowSynonym>
        <oboInOwl:hasNarrowSynonym>diclesium</oboInOwl:hasNarrowSynonym>
        <oboInOwl:hasNarrowSynonym>diplotegia</oboInOwl:hasNarrowSynonym>
        <oboInOwl:hasNarrowSynonym>diplotegium</oboInOwl:hasNarrowSynonym>
        <oboInOwl:hasNarrowSynonym>drupe</oboInOwl:hasNarrowSynonym>
        <oboInOwl:hasNarrowSynonym>folliceta</oboInOwl:hasNarrowSynonym>
        <oboInOwl:hasNarrowSynonym>follicetum</oboInOwl:hasNarrowSynonym>
        <oboInOwl:hasNarrowSynonym>follicle</oboInOwl:hasNarrowSynonym>
        <oboInOwl:hasNarrowSynonym>fruit</oboInOwl:hasNarrowSynonym>
        <oboInOwl:hasNarrowSynonym>glandes</oboInOwl:hasNarrowSynonym>
        <oboInOwl:hasNarrowSynonym>glans</oboInOwl:hasNarrowSynonym>
        <oboInOwl:hasNarrowSynonym>grain</oboInOwl:hasNarrowSynonym>
        <oboInOwl:hasNarrowSynonym>hesperidia</oboInOwl:hasNarrowSynonym>
        <oboInOwl:hasNarrowSynonym>hesperidium</oboInOwl:hasNarrowSynonym>
        <oboInOwl:hasNarrowSynonym>hip</oboInOwl:hasNarrowSynonym>
        <oboInOwl:hasNarrowSynonym>kernel</oboInOwl:hasNarrowSynonym>
        <oboInOwl:hasNarrowSynonym>legume</oboInOwl:hasNarrowSynonym>
        <oboInOwl:hasNarrowSynonym>loculicidal capsule</oboInOwl:hasNarrowSynonym>
        <oboInOwl:hasNarrowSynonym>loment</oboInOwl:hasNarrowSynonym>
        <oboInOwl:hasNarrowSynonym>lomentum</oboInOwl:hasNarrowSynonym>
        <oboInOwl:hasNarrowSynonym>multiple fruit</oboInOwl:hasNarrowSynonym>
        <oboInOwl:hasNarrowSynonym>nut</oboInOwl:hasNarrowSynonym>
        <oboInOwl:hasNarrowSynonym>nutlet</oboInOwl:hasNarrowSynonym>
        <oboInOwl:hasNarrowSynonym>pepo</oboInOwl:hasNarrowSynonym>
        <oboInOwl:hasNarrowSynonym>pod</oboInOwl:hasNarrowSynonym>
        <oboInOwl:hasNarrowSynonym>pome</oboInOwl:hasNarrowSynonym>
        <oboInOwl:hasNarrowSynonym>poricidal capsule</oboInOwl:hasNarrowSynonym>
        <oboInOwl:hasNarrowSynonym>pyxides</oboInOwl:hasNarrowSynonym>
        <oboInOwl:hasNarrowSynonym>pyxis</oboInOwl:hasNarrowSynonym>
        <oboInOwl:hasNarrowSynonym>samara</oboInOwl:hasNarrowSynonym>
        <oboInOwl:hasNarrowSynonym>schizocarp</oboInOwl:hasNarrowSynonym>
        <oboInOwl:hasNarrowSynonym>septicidal capsule</oboInOwl:hasNarrowSynonym>
        <oboInOwl:hasNarrowSynonym>septifragal capsule</oboInOwl:hasNarrowSynonym>
        <oboInOwl:hasNarrowSynonym>silicle</oboInOwl:hasNarrowSynonym>
        <oboInOwl:hasNarrowSynonym>silicula</oboInOwl:hasNarrowSynonym>
        <oboInOwl:hasNarrowSynonym>siliqua</oboInOwl:hasNarrowSynonym>
        <oboInOwl:hasNarrowSynonym>silique</oboInOwl:hasNarrowSynonym>
        <oboInOwl:hasNarrowSynonym>stone fruit</oboInOwl:hasNarrowSynonym>
        <oboInOwl:hasNarrowSynonym>syconia</oboInOwl:hasNarrowSynonym>
        <oboInOwl:hasNarrowSynonym>syconium</oboInOwl:hasNarrowSynonym>
        <oboInOwl:hasNarrowSynonym>syncarp</oboInOwl:hasNarrowSynonym>
        <oboInOwl:hasNarrowSynonym>utricle</oboInOwl:hasNarrowSynonym>
        <oboInOwl:hasOBONamespace>plant_anatomy</oboInOwl:hasOBONamespace>
        <oboInOwl:id>PO:0009001</oboInOwl:id>
        <oboInOwl:inSubset rdf:resource="http://purl.obolibrary.org/obo/po#Angiosperm"/>
        <oboInOwl:inSubset rdf:resource="http://purl.obolibrary.org/obo/po#Arabidopsis"/>
        <oboInOwl:inSubset rdf:resource="http://purl.obolibrary.org/obo/po#Maize"/>
        <oboInOwl:inSubset rdf:resource="http://purl.obolibrary.org/obo/po#Poaceae"/>
        <oboInOwl:inSubset rdf:resource="http://purl.obolibrary.org/obo/po#Rice"/>
        <oboInOwl:inSubset rdf:resource="http://purl.obolibrary.org/obo/po#TraitNet"/>
        <rdfs:comment>A fruit may contain additional plant structures (PO:0009011) that were part of a flower (PO:0009046) and mature along with the gynoecium, such as a receptacle (PO:0009064). A fruit may develop without fertilization in cases of parthenocarpy, apomixis, or other hormone-induced conditions and may not always contain seeds. Fruits only occur in angiosperms.</rdfs:comment>
        <rdfs:label>fruit</rdfs:label>
    </owl:Class>
    


    <!-- http://purl.obolibrary.org/obo/PO_0009005 -->

    <owl:Class rdf:about="http://purl.obolibrary.org/obo/PO_0009005">
        <rdfs:subClassOf rdf:resource="http://purl.obolibrary.org/obo/PO_0025004"/>
        <obo:IAO_0000115>A plant axis (PO:0025004) that is part of a root system (PO:0025025).</obo:IAO_0000115>
        <obo:IAO_0000412 rdf:resource="http://purl.obolibrary.org/obo/po.owl"/>
        <oboInOwl:hasAlternativeId>PO:0003006</oboInOwl:hasAlternativeId>
        <oboInOwl:hasExactSynonym>ra&amp;#237z (Spanish)</oboInOwl:hasExactSynonym>
        <oboInOwl:hasExactSynonym>radices</oboInOwl:hasExactSynonym>
        <oboInOwl:hasExactSynonym>radix</oboInOwl:hasExactSynonym>
        <oboInOwl:hasExactSynonym>根 (Japanese)</oboInOwl:hasExactSynonym>
        <oboInOwl:hasNarrowSynonym>aerial root</oboInOwl:hasNarrowSynonym>
        <oboInOwl:hasNarrowSynonym>climbing root</oboInOwl:hasNarrowSynonym>
        <oboInOwl:hasOBONamespace>plant_anatomy</oboInOwl:hasOBONamespace>
        <oboInOwl:id>PO:0009005</oboInOwl:id>
        <oboInOwl:inSubset rdf:resource="http://purl.obolibrary.org/obo/po#Maize"/>
        <oboInOwl:inSubset rdf:resource="http://purl.obolibrary.org/obo/po#TraitNet"/>
        <oboInOwl:inSubset rdf:resource="http://purl.obolibrary.org/obo/po#reference"/>
        <rdfs:comment>Commonly thought of as one of the three basic parts of the seed plant body. A plant stucture that is usually underground and does not bear leaves and only rarely shoots, is usually more or less positively geotropic, is endogenous in origin, indeterminate in growth and often with secondary thickening.</rdfs:comment>
        <rdfs:label>root</rdfs:label>
    </owl:Class>
    


    <!-- http://purl.obolibrary.org/obo/PO_0009008 -->

    <owl:Class rdf:about="http://purl.obolibrary.org/obo/PO_0009008">
        <rdfs:subClassOf rdf:resource="http://purl.obolibrary.org/obo/PO_0025496"/>
        <obo:IAO_0000115>A multi-tissue plant structure (PO:0025496) that is a functional unit, is a proper part of a whole plant (PO:0000003), and includes portions of plant tissue (PO:0009007) of at least two different types that derive from a common developmental path.</obo:IAO_0000115>
        <obo:IAO_0000412 rdf:resource="http://purl.obolibrary.org/obo/po.owl"/>
        <oboInOwl:hasBroadSynonym>organ</oboInOwl:hasBroadSynonym>
        <oboInOwl:hasDbXref>OBO_SF_PO:2932521</oboInOwl:hasDbXref>
        <oboInOwl:hasExactSynonym>&amp;#243rgano vegetal (Spanish)</oboInOwl:hasExactSynonym>
        <oboInOwl:hasExactSynonym>植物 器官 (Japanese)</oboInOwl:hasExactSynonym>
        <oboInOwl:hasOBONamespace>plant_anatomy</oboInOwl:hasOBONamespace>
        <oboInOwl:hasRelatedSynonym>compound plant organ</oboInOwl:hasRelatedSynonym>
        <oboInOwl:hasRelatedSynonym>simple plant organ</oboInOwl:hasRelatedSynonym>
        <oboInOwl:id>PO:0009008</oboInOwl:id>
        <oboInOwl:inSubset rdf:resource="http://purl.obolibrary.org/obo/po#TraitNet"/>
        <rdfs:comment>Examples include stem (PO:0009047), leaf (PO:0025034), and root (PO:0009005). May include individual plant cells (PO:0009002) that are not part of a portion of plant tissue (e.g., idioblasts, PO:0000283). A plant organ may have one or more different plant organs as parts, such as a sporophyll (PO:0009026) that may have as part a sporangium (PO:0025094) or a carpel (PO:0009030) that may have as part a plant ovule (PO:0020003).</rdfs:comment>
        <rdfs:label>plant organ</rdfs:label>
    </owl:Class>
    


    <!-- http://purl.obolibrary.org/obo/PO_0009009 -->

    <owl:Class rdf:about="http://purl.obolibrary.org/obo/PO_0009009">
        <rdfs:subClassOf rdf:resource="http://purl.obolibrary.org/obo/PO_0000003"/>
        <obo:IAO_0000115>A whole plant (PO:0000003) that participates in the plant embryo stage (PO:0007631).</obo:IAO_0000115>
        <obo:IAO_0000412 rdf:resource="http://purl.obolibrary.org/obo/po.owl"/>
        <oboInOwl:hasBroadSynonym>embryo</oboInOwl:hasBroadSynonym>
        <oboInOwl:hasDbXref>OBO_SF_PO:2982384</oboInOwl:hasDbXref>
        <oboInOwl:hasExactSynonym>embri&amp;#243n (Spanish)</oboInOwl:hasExactSynonym>
        <oboInOwl:hasExactSynonym>植物胚 (Japanese)</oboInOwl:hasExactSynonym>
        <oboInOwl:hasOBONamespace>plant_anatomy</oboInOwl:hasOBONamespace>
        <oboInOwl:hasRelatedSynonym>germ</oboInOwl:hasRelatedSynonym>
        <oboInOwl:id>PO:0009009</oboInOwl:id>
        <rdfs:comment>A plant embryo is generally formed after the first division of a plant zygote (PO:0000423), but in the case of a nucellar (adventitious) plant embryo (PO:0004537), somatic plant embryo (PO:0025302), microspore-derived cultured plant embryo (PO:0025305), and other embryos that arise through apogamy, it begins after the division of a single cell that is not a zygote. The end of the embryo stage varies among taxa; the beginning of a seed germination stage (PO:0007057) in seed plants, formation of the first vascular leaf (PO:0009025) in pteridophytes, the beginning of development of a sporangium (PO:0025094) in bryophytes, or the beginning of the formation of a plant organ (PO:0009008) such as a root (PO:0009005), shoot axis (PO:0025029), or vascular leaf (PO:0009025) in a cultured plant embryo (PO:0000010).</rdfs:comment>
        <rdfs:label>plant embryo</rdfs:label>
    </owl:Class>
    


    <!-- http://purl.obolibrary.org/obo/PO_0009010 -->

    <owl:Class rdf:about="http://purl.obolibrary.org/obo/PO_0009010">
        <rdfs:subClassOf rdf:resource="http://purl.obolibrary.org/obo/PO_0025496"/>
        <rdfs:subClassOf>
            <owl:Restriction>
                <owl:onProperty rdf:resource="http://purl.obolibrary.org/obo/BFO_0000051"/>
                <owl:someValuesFrom rdf:resource="http://purl.obolibrary.org/obo/PO_0009009"/>
            </owl:Restriction>
        </rdfs:subClassOf>
        <obo:IAO_0000115>A multi-tissue plant structure (PO:0025496) that develops from a plant ovule (PO:0020003) and has as parts a plant embryo (PO:0009009) enclosed in a seed coat (PO:0009088).</obo:IAO_0000115>
        <obo:IAO_0000412 rdf:resource="http://purl.obolibrary.org/obo/po.owl"/>
        <oboInOwl:hasBroadSynonym>diaspore</oboInOwl:hasBroadSynonym>
        <oboInOwl:hasDbXref>OBO_SF_PO:3458354</oboInOwl:hasDbXref>
        <oboInOwl:hasExactSynonym>semilla (Spanish)</oboInOwl:hasExactSynonym>
        <oboInOwl:hasExactSynonym>種子 (Japanese)</oboInOwl:hasExactSynonym>
        <oboInOwl:hasNarrowSynonym>pyrene</oboInOwl:hasNarrowSynonym>
        <oboInOwl:hasOBONamespace>plant_anatomy</oboInOwl:hasOBONamespace>
        <oboInOwl:id>PO:0009010</oboInOwl:id>
        <oboInOwl:inSubset rdf:resource="http://purl.obolibrary.org/obo/po#Angiosperm"/>
        <oboInOwl:inSubset rdf:resource="http://purl.obolibrary.org/obo/po#Arabidopsis"/>
        <oboInOwl:inSubset rdf:resource="http://purl.obolibrary.org/obo/po#Citrus"/>
        <oboInOwl:inSubset rdf:resource="http://purl.obolibrary.org/obo/po#Gymnosperms"/>
        <oboInOwl:inSubset rdf:resource="http://purl.obolibrary.org/obo/po#Maize"/>
        <oboInOwl:inSubset rdf:resource="http://purl.obolibrary.org/obo/po#Poaceae"/>
        <oboInOwl:inSubset rdf:resource="http://purl.obolibrary.org/obo/po#Rice"/>
        <oboInOwl:inSubset rdf:resource="http://purl.obolibrary.org/obo/po#Tomato"/>
        <oboInOwl:inSubset rdf:resource="http://purl.obolibrary.org/obo/po#TraitNet"/>
        <rdfs:comment>A seed generally develops from an ovule (PO:0020003) after fertilization, but may develop without fertilization in the case of apogamy (e.g., adventitious embryos or somatic embryos). A seed is a reproductive unit of seed plants (gymnosperms, angiosperms, and fossil pteridosperms).</rdfs:comment>
        <rdfs:label>seed</rdfs:label>
    </owl:Class>
    


    <!-- http://purl.obolibrary.org/obo/PO_0009011 -->

    <owl:Class rdf:about="http://purl.obolibrary.org/obo/PO_0009011">
        <rdfs:subClassOf rdf:resource="http://purl.obolibrary.org/obo/PO_0025131"/>
        <obo:IAO_0000115>An anatomical structure that is or was part of a plant, or was derived from a part of a plant.</obo:IAO_0000115>
        <obo:IAO_0000412 rdf:resource="http://purl.obolibrary.org/obo/po.owl"/>
        <oboInOwl:hasDbXref>OBO_SF_PO:2932527</oboInOwl:hasDbXref>
        <oboInOwl:hasExactSynonym>estructura vegetal (Spanish)</oboInOwl:hasExactSynonym>
        <oboInOwl:hasExactSynonym>植物 構造 (Japanese)</oboInOwl:hasExactSynonym>
        <oboInOwl:hasOBONamespace>plant_anatomy</oboInOwl:hasOBONamespace>
        <oboInOwl:id>PO:0009011</oboInOwl:id>
        <oboInOwl:inSubset rdf:resource="http://purl.obolibrary.org/obo/po#TraitNet"/>
        <rdfs:comment>&apos;Part&apos; includes both proper parts and the whole plant. CARO:0000003 anatomical structure is defined as: Material anatomical entity that has inherent 3D shape and is generated by coordinated expression of the organism&apos;s own genome.</rdfs:comment>
        <rdfs:label>plant structure</rdfs:label>
    </owl:Class>
    


    <!-- http://purl.obolibrary.org/obo/PO_0009047 -->

    <owl:Class rdf:about="http://purl.obolibrary.org/obo/PO_0009047">
        <rdfs:subClassOf rdf:resource="http://purl.obolibrary.org/obo/PO_0025029"/>
        <obo:IAO_0000115>A shoot axis (PO:0025029) that is the primary axis of a plant.</obo:IAO_0000115>
        <obo:IAO_0000412 rdf:resource="http://purl.obolibrary.org/obo/po.owl"/>
        <oboInOwl:hasDbXref>OBO_SF_PO:2903994</oboInOwl:hasDbXref>
        <oboInOwl:hasDbXref>OBO_SF_PO:2982923</oboInOwl:hasDbXref>
        <oboInOwl:hasExactSynonym>ca&amp;#241a (Spanish)</oboInOwl:hasExactSynonym>
        <oboInOwl:hasExactSynonym>culm</oboInOwl:hasExactSynonym>
        <oboInOwl:hasExactSynonym>eje primario (Spanish)</oboInOwl:hasExactSynonym>
        <oboInOwl:hasExactSynonym>primary axis</oboInOwl:hasExactSynonym>
        <oboInOwl:hasExactSynonym>primary stem</oboInOwl:hasExactSynonym>
        <oboInOwl:hasExactSynonym>tallo (Spanish)</oboInOwl:hasExactSynonym>
        <oboInOwl:hasExactSynonym>tronco (Spanish)</oboInOwl:hasExactSynonym>
        <oboInOwl:hasExactSynonym>茎 (Japanese)</oboInOwl:hasExactSynonym>
        <oboInOwl:hasNarrowSynonym>bole</oboInOwl:hasNarrowSynonym>
        <oboInOwl:hasNarrowSynonym>cane</oboInOwl:hasNarrowSynonym>
        <oboInOwl:hasNarrowSynonym>caudex</oboInOwl:hasNarrowSynonym>
        <oboInOwl:hasNarrowSynonym>caudices</oboInOwl:hasNarrowSynonym>
        <oboInOwl:hasNarrowSynonym>primocane</oboInOwl:hasNarrowSynonym>
        <oboInOwl:hasNarrowSynonym>scape</oboInOwl:hasNarrowSynonym>
        <oboInOwl:hasNarrowSynonym>stalk</oboInOwl:hasNarrowSynonym>
        <oboInOwl:hasNarrowSynonym>trunk</oboInOwl:hasNarrowSynonym>
        <oboInOwl:hasOBONamespace>plant_anatomy</oboInOwl:hasOBONamespace>
        <oboInOwl:id>PO:0009047</oboInOwl:id>
        <oboInOwl:inSubset rdf:resource="http://purl.obolibrary.org/obo/po#TraitNet"/>
        <oboInOwl:inSubset rdf:resource="http://purl.obolibrary.org/obo/po#reference"/>
        <rdfs:comment>Often bears leaves and buds. It is usually above ground, more or less negatively geotropic, and exogenous in origin.</rdfs:comment>
        <rdfs:label>stem</rdfs:label>
    </owl:Class>
    


    <!-- http://purl.obolibrary.org/obo/PO_0025004 -->

    <owl:Class rdf:about="http://purl.obolibrary.org/obo/PO_0025004">
        <rdfs:subClassOf rdf:resource="http://purl.obolibrary.org/obo/PO_0009008"/>
        <obo:IAO_0000115>An axial plant organ (PO:0009008).</obo:IAO_0000115>
        <obo:IAO_0000412 rdf:resource="http://purl.obolibrary.org/obo/po.owl"/>
        <oboInOwl:created_by>rwalls</oboInOwl:created_by>
        <oboInOwl:creation_date>2010-07-01T03:44:41Z</oboInOwl:creation_date>
        <oboInOwl:hasExactSynonym>eje de la planta (Spanish)</oboInOwl:hasExactSynonym>
        <oboInOwl:hasExactSynonym>plant axes</oboInOwl:hasExactSynonym>
        <oboInOwl:hasExactSynonym>植物軸（軸柱） (Japanese)</oboInOwl:hasExactSynonym>
        <oboInOwl:hasOBONamespace>plant_anatomy</oboInOwl:hasOBONamespace>
        <oboInOwl:id>PO:0025004</oboInOwl:id>
        <oboInOwl:inSubset rdf:resource="http://purl.obolibrary.org/obo/po#TraitNet"/>
        <rdfs:comment>Includes roots and shoots.</rdfs:comment>
        <rdfs:label>plant axis</rdfs:label>
    </owl:Class>
    


    <!-- http://purl.obolibrary.org/obo/PO_0025029 -->

    <owl:Class rdf:about="http://purl.obolibrary.org/obo/PO_0025029">
        <rdfs:subClassOf rdf:resource="http://purl.obolibrary.org/obo/PO_0025004"/>
        <obo:IAO_0000115>A plant axis (PO:0025004) that is part of a shoot system (PO:0009006).</obo:IAO_0000115>
        <obo:IAO_0000412 rdf:resource="http://purl.obolibrary.org/obo/po.owl"/>
        <oboInOwl:created_by>rwalls</oboInOwl:created_by>
        <oboInOwl:creation_date>2010-07-01T03:46:35Z</oboInOwl:creation_date>
        <oboInOwl:hasExactSynonym>caullome</oboInOwl:hasExactSynonym>
        <oboInOwl:hasExactSynonym>eje del epiblasto (epiblastema) (Spanish)</oboInOwl:hasExactSynonym>
        <oboInOwl:hasExactSynonym>シュート軸 (Japanese)</oboInOwl:hasExactSynonym>
        <oboInOwl:hasOBONamespace>plant_anatomy</oboInOwl:hasOBONamespace>
        <oboInOwl:hasRelatedSynonym>shoot</oboInOwl:hasRelatedSynonym>
        <oboInOwl:id>PO:0025029</oboInOwl:id>
        <oboInOwl:inSubset rdf:resource="http://purl.obolibrary.org/obo/po#TraitNet"/>
        <rdfs:comment>Often bears leaves and branches. In vascular plants, has at least one node and one internode.</rdfs:comment>
        <rdfs:label>shoot axis</rdfs:label>
    </owl:Class>
    


    <!-- http://purl.obolibrary.org/obo/PO_0025034 -->

    <owl:Class rdf:about="http://purl.obolibrary.org/obo/PO_0025034">
        <rdfs:subClassOf rdf:resource="http://purl.obolibrary.org/obo/PO_0006001"/>
        <obo:IAO_0000115>A phyllome (PO:0006001) that is not associated with a reproductive structure.</obo:IAO_0000115>
        <obo:IAO_0000412 rdf:resource="http://purl.obolibrary.org/obo/po.owl"/>
        <oboInOwl:created_by>rwalls</oboInOwl:created_by>
        <oboInOwl:creation_date>2010-07-12T01:31:44Z</oboInOwl:creation_date>
        <oboInOwl:hasDbXref>OBO_SF_PO:3167333</oboInOwl:hasDbXref>
        <oboInOwl:hasDbXref>OBO_SF_PO:3205370</oboInOwl:hasDbXref>
        <oboInOwl:hasExactSynonym>hoja (Spanish)</oboInOwl:hasExactSynonym>
        <oboInOwl:hasExactSynonym>葉 (Japanese)</oboInOwl:hasExactSynonym>
        <oboInOwl:hasOBONamespace>plant_anatomy</oboInOwl:hasOBONamespace>
        <oboInOwl:id>PO:0025034</oboInOwl:id>
        <oboInOwl:inSubset rdf:resource="http://purl.obolibrary.org/obo/po#TraitNet"/>
        <rdfs:label>leaf</rdfs:label>
    </owl:Class>
    


    <!-- http://purl.obolibrary.org/obo/PO_0025131 -->

    <owl:Class rdf:about="http://purl.obolibrary.org/obo/PO_0025131">
        <obo:IAO_0000115>An anatomical entity that is or was part of a plant.</obo:IAO_0000115>
        <obo:IAO_0000412 rdf:resource="http://purl.obolibrary.org/obo/po.owl"/>
        <oboInOwl:created_by>rwalls</oboInOwl:created_by>
        <oboInOwl:creation_date>2010-11-15T11:41:38Z</oboInOwl:creation_date>
        <oboInOwl:hasDbXref>OBO_SF_PO:3115810</oboInOwl:hasDbXref>
        <oboInOwl:hasExactSynonym>entidad anat&amp;#243mica vegetal (Spanish)</oboInOwl:hasExactSynonym>
        <oboInOwl:hasExactSynonym>植物 解剖学（形態）的実体 (Japanese)</oboInOwl:hasExactSynonym>
        <oboInOwl:hasOBONamespace>plant_anatomy</oboInOwl:hasOBONamespace>
        <oboInOwl:id>PO:0025131</oboInOwl:id>
        <rdfs:comment>Includes both material entities such as plant structures and immaterial entities such as plant anatomical spaces. CARO:0000000 anatomical entity is defined as: Biological entity that is either an individual member of a biological species or constitutes the structural organization of an individual member of a biological species.</rdfs:comment>
        <rdfs:label>plant anatomical entity</rdfs:label>
    </owl:Class>
    


    <!-- http://purl.obolibrary.org/obo/PO_0025496 -->

    <owl:Class rdf:about="http://purl.obolibrary.org/obo/PO_0025496">
        <rdfs:subClassOf rdf:resource="http://purl.obolibrary.org/obo/PO_0009011"/>
        <obo:IAO_0000115>A plant structure (PO:0009011) that has as parts two or more portions of plant tissue (PO:0009007) of at least two different types and which through specific morphogenetic processes forms a single structural unit demarcated by primarily bona-fide boundaries from other structural units of different types.</obo:IAO_0000115>
        <obo:IAO_0000412 rdf:resource="http://purl.obolibrary.org/obo/po.owl"/>
        <oboInOwl:created_by>cooperl</oboInOwl:created_by>
        <oboInOwl:creation_date>2012-06-11T14:57:00Z</oboInOwl:creation_date>
        <oboInOwl:hasDbXref>OBO_SF_PO:3530843</oboInOwl:hasDbXref>
        <oboInOwl:hasExactSynonym>estructura vegetal con m&amp;#250ltiples tejidos (Spanish)</oboInOwl:hasExactSynonym>
        <oboInOwl:hasExactSynonym>複数の組織からなる植物構造 (Japanese)</oboInOwl:hasExactSynonym>
        <oboInOwl:hasOBONamespace>plant_anatomy</oboInOwl:hasOBONamespace>
        <oboInOwl:id>PO:0025496</oboInOwl:id>
        <rdfs:comment>Most multi-tissue plant structures have at least a small connection to other plant structures via a fiat boundary, such as where a leaf (PO:0025034) connects to a shoot axis (PO:0025029), a petal (PO:0009032) connects to a receptacle (PO:0009064), or a branch (PO:0025073) connects to a stem (PO:0009047).</rdfs:comment>
        <rdfs:label>multi-tissue plant structure</rdfs:label>
    </owl:Class>
    


    <!-- http://purl.obolibrary.org/obo/PO_0025522 -->

    <owl:Class rdf:about="http://purl.obolibrary.org/obo/PO_0025522">
        <rdfs:subClassOf rdf:resource="http://purl.obolibrary.org/obo/PO_0025004"/>
        <obo:IAO_0000115>A plant axis (PO:0025004) that is radially enlarged.</obo:IAO_0000115>
        <obo:IAO_0000412 rdf:resource="http://purl.obolibrary.org/obo/po.owl"/>
        <oboInOwl:created_by>cooperl</oboInOwl:created_by>
        <oboInOwl:creation_date>2012-11-20T18:35:45Z</oboInOwl:creation_date>
        <oboInOwl:hasDbXref>OBO_SF_PO:3017726</oboInOwl:hasDbXref>
        <oboInOwl:hasExactSynonym>塊茎 (Japanese)</oboInOwl:hasExactSynonym>
        <oboInOwl:hasOBONamespace>plant_anatomy</oboInOwl:hasOBONamespace>
        <oboInOwl:id>PO:0025522</oboInOwl:id>
        <oboInOwl:inSubset rdf:resource="http://purl.obolibrary.org/obo/po#Potato"/>
        <rdfs:comment>Functions in storage of photosynthate metabolites. May develop from a branch (PO:0025073) or a root (PO:0009005).  If you are annotating to tuber, you should pick the more specific child term: shoot axis tuber (PO:0004543) or tuberous root tuber (PO:0025476).</rdfs:comment>
        <rdfs:label>tuber</rdfs:label>
    </owl:Class>
</rdf:RDF>



<!-- Generated by the OWL API (version 4.5.26) https://github.com/owlcs/owlapi -->

